ebstack finish

examples/Stacks/EBStack.v
@@ -71,6 +71,468 @@ Module EBStackImpl.
         Ret (match succ with | FAIL => inl tt | OK v => inr v end)
       end
     } Loop.
+
+  Definition assertion := @Assertion (@ProofState _ _ (li_lts E) (li_lts F)).
+  Definition rg_relation := @RGRelation _ _ (li_lts E) (li_lts F).
+
+  Open Scope rg_relation_scope.
+  Open Scope assertion_scope.
+
+  Definition stack_state (s : State (li_lts E)) : list A :=
+    state (fst s).
+
+  Definition exch_state (s : State (li_lts E)) : @EExchState (option A) :=
+    snd s.
+
+  Definition wait_lin (t : tid) (v : option A) (π : tmap Semantics.LinState) : Prop :=
+    match v with
+    | Some x => TMap.find t π = Some (Semantics.ls_inv (StackSpec.push x))
+    | None => TMap.find t π = Some (Semantics.ls_inv StackSpec.pop)
+    end.
+
+  Definition done_lin
+    (t : tid) (v other : option A) (π : tmap Semantics.LinState) : Prop :=
+    match v, other with
+    | Some x, None =>
+        TMap.find t π = Some (Semantics.ls_linr (StackSpec.push x) tt)
+    | None, Some x =>
+        TMap.find t π = Some (Semantics.ls_linr StackSpec.pop (Some x))
+    | _, _ => False
+    end.
+
+  Definition paired_lin
+    (t1 : tid) (v1 : option A) (t2 : tid) (v2 : option A)
+    (π : tmap Semantics.LinState) : Prop :=
+    match v1, v2 with
+    | Some _, None | None, Some _ =>
+        done_lin t1 v1 v2 π /\ done_lin t2 v2 v1 π
+    | Some _, Some _ | None, None =>
+        wait_lin t1 v1 π /\ wait_lin t2 v2 π
+    end.
+
+  Definition accepted_lin
+    (t1 : tid) (v1 : option A) (t2 : tid) (v2 : option A)
+    (π : tmap Semantics.LinState) : Prop :=
+    match v1, v2 with
+    | Some _, None | None, Some _ => done_lin t2 v2 v1 π
+    | Some _, Some _ | None, None => wait_lin t2 v2 π
+    end.
+
+  Definition exch_ok (xs : @EExchState (option A)) (π : tmap Semantics.LinState) : Prop :=
+    match xs with
+    | ExSIdle => True
+    | ExSOffered t v => wait_lin t v π
+    | ExSPaired t1 v1 t2 v2 => paired_lin t1 v1 t2 v2 π
+    | ExSAccepted t1 v1 t2 v2 => accepted_lin t1 v1 t2 v2 π
+    end.
+
+  Definition exch_distinct (xs : @EExchState (option A)) : Prop :=
+    match xs with
+    | ExSPaired t1 _ t2 _ | ExSAccepted t1 _ t2 _ => t1 <> t2
+    | _ => True
+    end.
+
+  Definition I : assertion :=
+    fun s =>
+      ρ s = Idle (stack_state (σ s)) /\
+      exch_ok (exch_state (σ s)) (π s) /\
+      exch_distinct (exch_state (σ s)).
+
+  Definition no_exch_by (t : tid) (xs : @EExchState (option A)) : Prop :=
+    match xs with
+    | ExSIdle => True
+    | ExSOffered t1 _ => t <> t1
+    | ExSPaired t1 _ t2 _ => t <> t1 /\ t <> t2
+    | ExSAccepted _ _ t2 _ => t <> t2
+    end.
+
+  Definition NoExchBy (t : tid) : assertion :=
+    fun s => no_exch_by t (exch_state (σ s)).
+
+  Definition Active (t : tid) (m : Sig.op (li_sig F)) : assertion :=
+    ALin t (Semantics.ls_inv m) //\\ NoExchBy t.
+
+  Definition Done (t : tid) (m : Sig.op (li_sig F)) : assertion :=
+    ∃ ret, ALin t (Semantics.ls_linr m ret).
+
+  Definition Live (t : tid) (m : Sig.op (li_sig F)) : assertion :=
+    ALin t (Semantics.ls_inv m) \\// Done t m.
+
+  Definition R_pres t : rg_relation :=
+    fun s1 s2 =>
+      (TMap.find t (π s1) = None <-> TMap.find t (π s2) = None) /\
+      (forall m, Active t m s1 -> Active t m s2) /\
+      (forall m ret, ALin t (Semantics.ls_linr m ret) s1 ->
+        ALin t (Semantics.ls_linr m ret) s2) /\
+      (forall m, Live t m s1 -> Live t m s2) /\
+      (NoExchBy t s1 -> NoExchBy t s2).
+
+  Definition G t : rg_relation :=
+    fun s1 s2 =>
+      I s2 /\
+      (forall t', t <> t' -> R_pres t' s1 s2).
+
+  Definition R t : rg_relation :=
+    R_pres t.
+
+  Lemma Istable {t} : Stable (R t) I I.
+  Proof. unfold Stable. apply ConjRightImpl, ImplRefl. Qed.
+
+  Lemma Activestable {t m}: Stable (R t) I (Active t m).
+  Proof.
+    unfold Stable, R, R_pres.
+    intros ? [[? [Hact [_ [Hpres _]]]] ?].
+    eauto.
+  Qed.
+
+  Lemma Donestable {t m}: Stable (R t) I (Done t m).
+  Proof.
+    unfold Stable, R, R_pres, Done.
+    intros ? [[? [[ret Hdone] [_ [_ [Hpres _]]]]] ?].
+    exists ret. eauto.
+  Qed.
+
+  Lemma ALinRetstable {t m ret}: Stable (R t) I (ALin t (Semantics.ls_linr m ret)).
+  Proof.
+    unfold Stable, R, R_pres.
+    intros ? [[? [Hdone [_ [_ [Hpres _]]]]] ?].
+    eauto.
+  Qed.
+
+  Lemma Livestable {t m}: Stable (R t) I (Live t m).
+  Proof.
+    unfold Stable, R, R_pres.
+    intros ? [[? [Hlive [_ [_ [_ [Hpres _]]]]]] ?].
+    eauto.
+  Qed.
+
+  Lemma NoExchBystable {t}: Stable (R t) I (NoExchBy t).
+  Proof.
+    unfold Stable, R, R_pres.
+    intros ? [[? [Hno [_ [_ [_ [_ Hpres]]]]]] ?].
+    eauto.
+  Qed.
+
+  Create HintDb stableDB.
+  Hint Resolve Istable Activestable Donestable ALinRetstable Livestable NoExchBystable : stableDB.
+
+  Lemma wait_lin_add_fresh t t' v f π :
+    TMap.find t π = None ->
+    wait_lin t' v π ->
+    wait_lin t' v (TMap.add t (Semantics.ls_inv f) π).
+  Proof.
+    intros Hnone Hwait.
+    destruct v; simpl in *;
+    destruct (PositiveMap.E.eq_dec t t'); subst.
+    - rewrite Hnone in Hwait. discriminate.
+    - rewrite PositiveMap.gso by auto. exact Hwait.
+    - rewrite Hnone in Hwait. discriminate.
+    - rewrite PositiveMap.gso by auto. exact Hwait.
+  Qed.
+
+  Lemma done_lin_add_fresh t t' v other f π :
+    TMap.find t π = None ->
+    done_lin t' v other π ->
+    done_lin t' v other (TMap.add t (Semantics.ls_inv f) π).
+  Proof.
+    intros Hnone Hdone.
+    destruct v as [v|], other as [other|]; simpl in *; try contradiction;
+    destruct (PositiveMap.E.eq_dec t t'); subst.
+    - rewrite Hnone in Hdone. discriminate.
+    - rewrite PositiveMap.gso by auto. exact Hdone.
+    - rewrite Hnone in Hdone. discriminate.
+    - rewrite PositiveMap.gso by auto. exact Hdone.
+  Qed.
+
+  Lemma paired_lin_add_fresh t t1 v1 t2 v2 f π :
+    TMap.find t π = None ->
+    paired_lin t1 v1 t2 v2 π ->
+    paired_lin t1 v1 t2 v2 (TMap.add t (Semantics.ls_inv f) π).
+  Proof.
+    destruct v1 as [a|], v2 as [b|]; simpl in *; intros Hnone [H1 H2]; split.
+    - change (wait_lin t1 (Some a) (TMap.add t (Semantics.ls_inv f) π)).
+      eapply wait_lin_add_fresh; eauto.
+    - change (wait_lin t2 (Some b) (TMap.add t (Semantics.ls_inv f) π)).
+      eapply wait_lin_add_fresh; eauto.
+    - change (done_lin t1 (Some a) None (TMap.add t (Semantics.ls_inv f) π)).
+      eapply done_lin_add_fresh; eauto.
+    - change (done_lin t2 None (Some a) (TMap.add t (Semantics.ls_inv f) π)).
+      eapply done_lin_add_fresh; eauto.
+    - change (done_lin t1 None (Some b) (TMap.add t (Semantics.ls_inv f) π)).
+      eapply done_lin_add_fresh; eauto.
+    - change (done_lin t2 (Some b) None (TMap.add t (Semantics.ls_inv f) π)).
+      eapply done_lin_add_fresh; eauto.
+    - change (wait_lin t1 None (TMap.add t (Semantics.ls_inv f) π)).
+      eapply wait_lin_add_fresh; eauto.
+    - change (wait_lin t2 None (TMap.add t (Semantics.ls_inv f) π)).
+      eapply wait_lin_add_fresh; eauto.
+  Qed.
+
+  Lemma accepted_lin_add_fresh t t1 v1 t2 v2 f π :
+    TMap.find t π = None ->
+    accepted_lin t1 v1 t2 v2 π ->
+    accepted_lin t1 v1 t2 v2 (TMap.add t (Semantics.ls_inv f) π).
+  Proof.
+    destruct v1 as [a|], v2 as [b|]; simpl in *; intros Hnone H.
+    - change (wait_lin t2 (Some b) (TMap.add t (Semantics.ls_inv f) π)).
+      eapply wait_lin_add_fresh; eauto.
+    - change (done_lin t2 None (Some a) (TMap.add t (Semantics.ls_inv f) π)).
+      eapply done_lin_add_fresh; eauto.
+    - change (done_lin t2 (Some b) None (TMap.add t (Semantics.ls_inv f) π)).
+      eapply done_lin_add_fresh; eauto.
+    - change (wait_lin t2 None (TMap.add t (Semantics.ls_inv f) π)).
+      eapply wait_lin_add_fresh; eauto.
+  Qed.
+
+  Lemma IGinv : forall t f, ⊨ Ginv t f ⊚ I ==>> I //\\ ALin t (Semantics.ls_inv f).
+  Proof.
+    unfold I, ALin, Ginv, LiftRelation_π.
+    intros t f s [s' [HI [? [? [Hnone Hπ]]]]].
+    destruct s, s'; simpl in *; subst.
+    split.
+    - destruct HI as [Hr [Hex Hdist]]. split; [exact Hr|].
+      split.
+      2:{ destruct σ0 as [ts xs]; simpl in *; exact Hdist. }
+      destruct σ0 as [ts xs]; simpl in *.
+      destruct xs as [ot ov|pt1 pv1 pt2 pv2|at1 av1 at2 av2|]; simpl in *; auto.
+      + eapply wait_lin_add_fresh; eauto.
+      + eapply paired_lin_add_fresh; eauto.
+      + eapply accepted_lin_add_fresh; eauto.
+    - simpl. rewrite PositiveMap.gss. auto.
+  Qed.
+
+  Lemma exch_ok_no_exch_add_fresh t xs π :
+    TMap.find t π = None ->
+    exch_ok xs π ->
+    no_exch_by t xs.
+  Proof.
+    intros Hnone Hex.
+    destruct xs as [t1 v1|t1 v1 t2 v2|t1 v1 t2 v2|]; simpl in *; auto.
+    - destruct v1; simpl in *; intros Heq; subst; rewrite Hnone in Hex; discriminate.
+    - destruct v1 as [a|], v2 as [b|]; simpl in *; destruct Hex as [H1 H2]; split;
+      intros Heq; subst; rewrite Hnone in *; discriminate.
+    - destruct v1 as [a|], v2 as [b|]; simpl in *;
+      intros Heq; subst; rewrite Hnone in Hex; discriminate.
+  Qed.
+
+  Lemma IGinvActive : forall t f, ⊨ Ginv t f ⊚ I ==>> I //\\ Active t f.
+  Proof.
+    unfold I, Active, ALin, NoExchBy, Ginv, LiftRelation_π.
+    intros t f s [s' [HI [? [? [Hnone Hπ]]]]].
+    destruct s, s'; simpl in *; subst.
+    destruct HI as [Hr [Hex Hdist]].
+    split.
+    - split; [exact Hr|].
+      split.
+      2:{ destruct σ0 as [ts xs]; simpl in *; exact Hdist. }
+      destruct σ0 as [ts xs]; simpl in *.
+      destruct xs as [ot ov|pt1 pv1 pt2 pv2|at1 av1 at2 av2|]; simpl in *; auto.
+      + eapply wait_lin_add_fresh; eauto.
+      + eapply paired_lin_add_fresh; eauto.
+      + eapply accepted_lin_add_fresh; eauto.
+    - split.
+      + simpl. rewrite PositiveMap.gss. auto.
+      + simpl. eapply exch_ok_no_exch_add_fresh; eauto.
+  Qed.
+
+  Lemma exch_ok_remove_no_exch t xs π :
+    no_exch_by t xs ->
+    exch_ok xs π ->
+    exch_ok xs (TMap.remove t π).
+  Proof.
+    intros Hno Hex.
+    destruct xs as [t1 v1|t1 v1 t2 v2|t1 v1 t2 v2|]; simpl in *; auto.
+    - destruct v1; simpl in *; rewrite PositiveMap.gro by auto; exact Hex.
+    - destruct v1 as [a|], v2 as [b|]; simpl in *; destruct Hex as [H1 H2]; destruct Hno as [Hn1 Hn2]; split;
+      rewrite PositiveMap.gro by auto; assumption.
+    - destruct v1 as [a|], v2 as [b|]; simpl in *;
+      rewrite PositiveMap.gro by auto; assumption.
+  Qed.
+
+  Lemma exch_ok_add_add_no_exch t xs π ls1 ls2 :
+    no_exch_by t xs ->
+    exch_ok xs π ->
+    exch_ok xs (TMap.add t ls2 (TMap.add t ls1 π)).
+  Proof.
+    intros Hno Hex.
+    destruct xs as [t1 v1|t1 v1 t2 v2|t1 v1 t2 v2|]; simpl in *; auto.
+    - destruct v1; simpl in *; repeat (rewrite PositiveMap.gso by auto); exact Hex.
+    - destruct v1 as [a|], v2 as [b|]; simpl in *; destruct Hex as [H1 H2]; destruct Hno as [Hn1 Hn2]; split;
+      repeat (rewrite PositiveMap.gso by auto); assumption.
+    - destruct v1 as [a|], v2 as [b|]; simpl in *;
+      repeat (rewrite PositiveMap.gso by auto); assumption.
+  Qed.
+
+  Lemma IGretNoExch : forall t f ret,
+    ⊨ Gret t f ret ⊚ (I //\\ ALin t (Semantics.ls_linr f ret) //\\ NoExchBy t) ==>> I.
+  Proof.
+    unfold Gret, LiftRelation_π.
+    intros t f ret s [s' [Hpre [? [? [Hfind Hπ]]]]].
+    destruct Hpre as [HI [Hlin Hno]].
+    unfold I, ALin, NoExchBy in *.
+    destruct s, s'; simpl in *; subst.
+    destruct HI as [Hr [Hex Hdist]]. split; [exact Hr|].
+    destruct σ0 as [ts xs]; simpl in *.
+    split.
+    - eapply exch_ok_remove_no_exch; eauto.
+    - exact Hdist.
+  Qed.
+
+  Lemma no_error t (m : Sig.op (li_sig E)) (P : assertion) :
+    ⊨ P ==>> ANoError {| te_tid := t; te_ev := InvEv m |}.
+  Proof.
+    unfold ANoError.
+    intros [σ0 ρ0 π0] _ Herr.
+    destruct σ0 as [ts xs], m as [m|m]; simpl in *; contradiction.
+  Qed.
+
+  Lemma R_pres_ginv_other t t' f s1 s2 :
+    t <> t' ->
+    Ginv t f s1 s2 ->
+    R_pres t' s1 s2.
+  Proof.
+    intros Hneq Hinv.
+    assert (Hneq' : t' <> t) by congruence.
+    unfold Ginv, LiftRelation_π in Hinv.
+    destruct s1 as [σ1 ρ1 π1], s2 as [σ2 ρ2 π2]; simpl in *.
+    destruct Hinv as [Hσ [Hρ [Hfind Hπ]]]. subst.
+    unfold R_pres, Active, NoExchBy, Live, Done, ALin; simpl.
+    split.
+    - split; intro H.
+      + rewrite (@PositiveMap.gso Semantics.LinState t' t (Semantics.ls_inv f) π1 Hneq'). exact H.
+      + rewrite (@PositiveMap.gso Semantics.LinState t' t (Semantics.ls_inv f) π1 Hneq') in H. exact H.
+    - split.
+      + intros m [Hlin Hno]. simpl in *. split.
+        * change (TMap.find t' (TMap.add t (Semantics.ls_inv f) π1) =
+            Some (Semantics.ls_inv m)).
+          rewrite (@PositiveMap.gso Semantics.LinState t' t (Semantics.ls_inv f) π1 Hneq').
+          exact Hlin.
+        * exact Hno.
+      + split.
+        * intros m ret H. simpl in *.
+          change (TMap.find t' (TMap.add t (Semantics.ls_inv f) π1) =
+            Some (Semantics.ls_linr m ret)).
+          rewrite (@PositiveMap.gso Semantics.LinState t' t (Semantics.ls_inv f) π1 Hneq').
+          exact H.
+        * split.
+          -- intros m [Hlin | [ret Hret]]; simpl in *; simpl.
+             ++ left.
+                change (TMap.find t' (TMap.add t (Semantics.ls_inv f) π1) =
+                  Some (Semantics.ls_inv m)).
+                rewrite (@PositiveMap.gso Semantics.LinState t' t (Semantics.ls_inv f) π1 Hneq').
+                exact Hlin.
+             ++ right. exists ret.
+                change (TMap.find t' (TMap.add t (Semantics.ls_inv f) π1) =
+                  Some (Semantics.ls_linr m ret)).
+                rewrite (@PositiveMap.gso Semantics.LinState t' t (Semantics.ls_inv f) π1 Hneq').
+                exact Hret.
+          -- intros H. exact H.
+  Qed.
+
+  Lemma R_pres_gret_other t t' f ret s1 s2 :
+    t <> t' ->
+    Gret t f ret s1 s2 ->
+    R_pres t' s1 s2.
+  Proof.
+    intros Hneq Hret.
+    assert (Hneq' : t' <> t) by congruence.
+    unfold Gret, LiftRelation_π in Hret.
+    destruct s1 as [σ1 ρ1 π1], s2 as [σ2 ρ2 π2]; simpl in *.
+    destruct Hret as [Hσ [Hρ [Hfind Hπ]]]. subst.
+    unfold R_pres, Active, NoExchBy, Live, Done, ALin; simpl.
+    split.
+    - split; intro H.
+      + rewrite (@PositiveMap.gro Semantics.LinState t' t π1 Hneq'). exact H.
+      + rewrite (@PositiveMap.gro Semantics.LinState t' t π1 Hneq') in H. exact H.
+    - split.
+      + intros m [Hlin Hno]. simpl in *. split.
+        * change (TMap.find t' (TMap.remove t π1) =
+            Some (Semantics.ls_inv m)).
+          rewrite (@PositiveMap.gro Semantics.LinState t' t π1 Hneq').
+          exact Hlin.
+        * exact Hno.
+      + split.
+        * intros m r H. simpl in *.
+          change (TMap.find t' (TMap.remove t π1) =
+            Some (Semantics.ls_linr m r)).
+          rewrite (@PositiveMap.gro Semantics.LinState t' t π1 Hneq').
+          exact H.
+        * split.
+          -- intros m [Hlin | [r Hr]]; simpl in *; simpl.
+             ++ left.
+                change (TMap.find t' (TMap.remove t π1) =
+                  Some (Semantics.ls_inv m)).
+                rewrite (@PositiveMap.gro Semantics.LinState t' t π1 Hneq').
+                exact Hlin.
+             ++ right. exists r.
+                change (TMap.find t' (TMap.remove t π1) =
+                  Some (Semantics.ls_linr m r)).
+                rewrite (@PositiveMap.gro Semantics.LinState t' t π1 Hneq').
+                exact Hr.
+          -- intros H. exact H.
+  Qed.
+
+  Lemma R_pres_refl t s : R_pres t s s.
+  Proof.
+    unfold R_pres. firstorder.
+  Qed.
+
+  Lemma R_pres_same_π t' σ1 σ2 ρ0 π0 :
+    (no_exch_by t' (exch_state σ1) -> no_exch_by t' (exch_state σ2)) ->
+    R_pres t' (σ1, ρ0, π0) (σ2, ρ0, π0).
+  Proof.
+    unfold R_pres, Active, Live, Done, ALin, NoExchBy.
+    simpl. intros Hno.
+    split; [tauto|].
+    split.
+    - intros m [Hlin Hnx]. split; [exact Hlin|auto].
+    - split.
+      + intros m ret Hlin. exact Hlin.
+      + split.
+        * intros m Hlive. exact Hlive.
+        * intros Hnx. auto.
+  Qed.
+
+  Lemma R_pres_add_add_other t t' ls1 ls2 σ1 σ2 ρ1 ρ2 π0 :
+    t <> t' ->
+    (no_exch_by t' (exch_state σ1) -> no_exch_by t' (exch_state σ2)) ->
+    R_pres t' (σ1, ρ1, π0) (σ2, ρ2, TMap.add t ls2 (TMap.add t ls1 π0)).
+  Proof.
+    intros Hneq Hno.
+    assert (Hneq' : t' <> t) by congruence.
+    unfold R_pres, Active, Live, Done, ALin, NoExchBy.
+    simpl.
+    split.
+    - split; intro Hnone.
+      + rewrite PositiveMap.gso by exact Hneq'.
+        rewrite PositiveMap.gso by exact Hneq'.
+        exact Hnone.
+      + rewrite PositiveMap.gso in Hnone by exact Hneq'.
+        rewrite PositiveMap.gso in Hnone by exact Hneq'.
+        exact Hnone.
+    - split.
+      + intros m [Hlin Hnx]. simpl in *. split.
+        * simpl. rewrite PositiveMap.gso by exact Hneq'.
+          rewrite PositiveMap.gso by exact Hneq'.
+          exact Hlin.
+        * auto.
+      + split.
+        * intros m ret Hlin. simpl in *.
+          simpl. rewrite PositiveMap.gso by exact Hneq'.
+          rewrite PositiveMap.gso by exact Hneq'.
+          exact Hlin.
+        * split.
+          -- intros m [Hlin | [ret Hlin]]; simpl in *.
+             ++ left. simpl.
+                rewrite PositiveMap.gso by exact Hneq'.
+                rewrite PositiveMap.gso by exact Hneq'.
+                exact Hlin.
+             ++ right. exists ret. simpl.
+                rewrite PositiveMap.gso by exact Hneq'.
+                rewrite PositiveMap.gso by exact Hneq'.
+                exact Hlin.
+          -- intros Hnx. auto.
+  Qed.
     
   Program Definition Mebstack : layer_implementation E F := {|
     li_impl m :=
@@ -79,5 +541,867 @@ Module EBStackImpl.
       | pop => pop_impl
       end
   |}.
-  (* TODO: *)
-End TreiberStackImpl.
+  Next Obligation.
+    eapply RGILogic.soundness with (R:=R) (G:=G) (I:=I).
+	    {
+	      constructor.
+	      unfold R. intros s s' Hrel _.
+	      exact (proj1 Hrel).
+	    }
+	    {
+	      unfold G, R.
+	      intros t1 t2 Hneq s1 s2 Hrel.
+	      destruct Hrel as [HG | Hmeta].
+	      - exact (proj2 HG t2 Hneq).
+	      - unfold GINV, GRET, GId in Hmeta.
+	        destruct Hmeta as [[Hinv | Hret] | Hid].
+	        + destruct Hinv as [f Hinv].
+	          eapply R_pres_ginv_other; eauto.
+	        + destruct Hret as [f [ret Hret]].
+	          eapply R_pres_gret_other; eauto.
+	        + subst. apply R_pres_refl.
+	    }
+    intros t f. destruct f.
+    - exists (I //\\ Active t (push v)).
+      exists (fun _ => I //\\ ALin t (Semantics.ls_linr (push v) tt) //\\ NoExchBy t).
+      constructor.
+      + apply IGinvActive.
+      + solve_conj_impl.
+      + solve_conj_stable stableDB.
+      + intros [].
+        apply IGretNoExch.
+      + unfold ALin. intros [] σ0 ρ0 π0 [HI [Hlin Hno]].
+        exact Hlin.
+      + simpl. unfold push_impl.
+        eapply provable_doloop;
+        try solve_conj_impl;
+        try solve_conj_stable stableDB.
+        eapply provable_vis_safe with
+          (P' := I //\\ Live t (push v))
+          (Q' := fun other =>
+            match other with
+            | Some None => I //\\ ALin t (Semantics.ls_linr (push v) tt) //\\ NoExchBy t
+            | _ => I //\\ Active t (push v)
+            end);
+        try solve_conj_impl;
+        try solve_conj_stable stableDB;
+        try (intro other; destruct other as [[ov|]|]; try destruct ov; solve_conj_stable stableDB);
+        try solve [apply no_error].
+        * intros [[ov|]|]; try destruct ov; solve_conj_impl.
+        * pupdate_intros_atomic.
+          {
+            pupdate_finish; split.
+            - destruct Hpre as [HI [Hlin Hno]].
+              unfold I, Active, Live, Done, ALin, NoExchBy in *; simpl in *.
+              split.
+              + destruct HI as [Hr _]. split; [exact Hr|split; [exact Hlin|auto]].
+              + left. exact Hlin.
+            - unfold G, R_pres, Active, Live, Done, ALin, NoExchBy.
+              split.
+              + destruct Hpre as [HI [Hlin Hno]].
+                unfold I in *; simpl in *.
+                destruct HI as [Hr _]. split; [exact Hr|split; [exact Hlin|auto]].
+              + intros t' Hneq; simpl.
+                split.
+                -- split; intro H; exact H.
+                -- split.
+                   ++ intros m [Hlin Hno]. split; [exact Hlin|congruence].
+                   ++ split.
+                      ** intros m ret Hlin. exact Hlin.
+                      ** split.
+                         --- intros m [Hlin | [ret Hlin]]; [left | right; exists ret]; exact Hlin.
+                         --- intros _. congruence.
+          }
+          {
+            destruct v1 as [w|].
+            - pupdate_finish; split.
+              + destruct Hpre as [HI [Hlin Hno]].
+	                unfold I, Active, Live, Done, ALin, NoExchBy in *; simpl in *.
+		                destruct HI as [Hr [Hex Hdist]].
+		                split; [split; [exact Hr|split; [split; [exact Hex|exact Hlin]|congruence]]|left; exact Hlin].
+              + unfold G, R_pres, Active, Live, Done, ALin, NoExchBy.
+                split.
+                * destruct Hpre as [HI [Hlin Hno]].
+                  unfold I, Active, ALin in *; simpl in *.
+		                  destruct HI as [Hr [Hex Hdist]].
+		                  split; [exact Hr|split; [split; [exact Hex|exact Hlin]|congruence]].
+	                * intros t' Hneq; simpl.
+                  destruct (PositiveMap.E.eq_dec t' t1) as [Heq|Hne1]; subst.
+                  -- split.
+                     ++ split; intro Hnone.
+                        ** destruct Hpre as [HI [Hlin Hno]].
+                           unfold I in HI; simpl in HI.
+	                           destruct HI as [_ [Hex _]].
+                           rewrite Hex in Hnone. discriminate.
+                        ** destruct Hpre as [HI [Hlin Hno]].
+                           unfold I in HI; simpl in HI.
+	                           destruct HI as [_ [Hex _]].
+                           rewrite Hex in Hnone. discriminate.
+                     ++ split.
+                        ** intros m [Hlin Hno]. contradiction.
+                        ** split.
+                           --- intros m ret Hret.
+                               destruct Hpre as [HI _].
+                               unfold I in HI; simpl in HI.
+	                               destruct HI as [_ [Hex _]].
+                               rewrite Hex in Hret. discriminate.
+                           --- split.
+	                               +++ intros m [Hlin | [ret Hret]].
+                                   { left; exact Hlin. }
+                                   { destruct Hpre as [HI _].
+                                     unfold I in HI; simpl in HI.
+	                                     destruct HI as [_ [Hex _]].
+                                     simpl in Hret.
+                                     rewrite Hex in Hret. discriminate. }
+                               +++ intros Hno. contradiction.
+                  -- split.
+                     ++ split; intro Hnone; exact Hnone.
+                     ++ split.
+                        ** intros m [Hlin Hno]. split; [exact Hlin|split; [exact Hno|congruence]].
+                        ** split.
+                           --- intros m ret Hret. exact Hret.
+                           --- split.
+                               +++ intros m [Hlin | [ret Hret]]; [left | right; exists ret]; exact Hlin || exact Hret.
+                               +++ intros Hno. split; [exact Hno|congruence].
+	            - destruct Hpre as [HI [Hlin Hno]].
+                unfold I, Active, ALin, NoExchBy in *; simpl in *.
+                destruct HI as [Hr [Hex Hdist]]. subst ρ1.
+                pupdate_start.
+                pupdate_forward t2 (InvEv (push v)).
+                pupdate_forward t2 (ResEv (push v) tt).
+                pupdate_forward t1 (@InvEv (EStack A) (@pop A));
+                  try (rewrite PositiveMap.gso by congruence;
+                       rewrite PositiveMap.gso by congruence;
+                       exact Hex).
+                pupdate_forward t1 (@ResEv (EStack A) (@pop A) (Some v)).
+                pupdate_finish.
+                split.
+	                + split.
+	                  * split; [reflexivity|].
+	                    simpl. split.
+	                    -- split.
+                         ++ rewrite PositiveMap.gss. reflexivity.
+                         ++ rewrite PositiveMap.gso by congruence.
+                            rewrite PositiveMap.gso by congruence.
+                            rewrite PositiveMap.gss. reflexivity.
+	                    -- congruence.
+	                  * right. exists tt.
+	                    unfold ALin; simpl.
+                    rewrite PositiveMap.gso by congruence.
+                    rewrite PositiveMap.gso by congruence.
+                    rewrite PositiveMap.gss. reflexivity.
+                + unfold G, R_pres, Active, Live, Done, ALin, NoExchBy.
+                  split.
+	                  * split; [reflexivity|].
+	                    simpl. split.
+	                    -- split.
+                         ++ rewrite PositiveMap.gss. reflexivity.
+                         ++ rewrite PositiveMap.gso by congruence.
+                            rewrite PositiveMap.gso by congruence.
+                            rewrite PositiveMap.gss. reflexivity.
+	                    -- congruence.
+                  * intros t' Hneq.
+                    simpl.
+                    destruct (PositiveMap.E.eq_dec t' t1) as [Heq|Hne1]; subst.
+                    -- split.
+                       ++ split; intro Hnone.
+                          ** rewrite Hex in Hnone. discriminate.
+                          ** rewrite PositiveMap.gss in Hnone. discriminate.
+                       ++ split.
+                          ** intros m [Hinv Hno']. contradiction.
+                          ** split.
+                             --- intros m ret Hret.
+                                 rewrite Hex in Hret. discriminate.
+                             --- split.
+	                                 +++ intros m [Hinv | [ret Hret]].
+	                                     { destruct m as [x|].
+                                         - simpl in Hinv. rewrite Hex in Hinv. discriminate.
+                                         - right. exists (Some v).
+                                           simpl. rewrite PositiveMap.gss. reflexivity. }
+	                                     { simpl in Hret. rewrite Hex in Hret. discriminate. }
+                                 +++ intros Hno'. contradiction.
+	                    -- assert (Hne2 : t' <> t2) by congruence.
+                       simpl in *.
+	                       split.
+                       ++ split; intro Hnone.
+                          ** repeat (rewrite PositiveMap.gso by congruence). exact Hnone.
+                          ** repeat (rewrite PositiveMap.gso in Hnone by congruence). exact Hnone.
+                       ++ split.
+	                          ** intros m [Hinv Hno']. simpl in Hinv. split.
+	                             --- simpl. repeat (rewrite PositiveMap.gso by congruence). exact Hinv.
+                             --- split; [exact Hno'|exact Hne2].
+                          ** split.
+	                             --- intros m ret Hret. simpl in Hret.
+	                                 simpl. repeat (rewrite PositiveMap.gso by congruence). exact Hret.
+                             --- split.
+	                                 +++ intros m [Hinv | [ret Hret]].
+	                                     { simpl in Hinv. left. simpl. repeat (rewrite PositiveMap.gso by congruence). exact Hinv. }
+	                                     { simpl in Hret. right. exists ret. simpl. repeat (rewrite PositiveMap.gso by congruence). exact Hret. }
+	                                 +++ intros Hno'. split; [exact Hno'|exact Hne2].
+	          }
+        * intros ret.
+          pupdate_intros_atomic.
+	          { inversion H0; subst; clear H0.
+	            pupdate_finish; split.
+            + destruct Hpre as [HI Hlive].
+              unfold I, Live, Done, ALin in *; simpl in *.
+              destruct HI as [Hr [Hex Hdist]]. subst ρ1.
+              split; [split; [reflexivity|split; auto]|].
+              split; [exact Hex|auto].
+            + unfold G. split.
+              * destruct Hpre as [HI Hlive].
+                unfold I in *; simpl in *.
+                destruct HI as [Hr [Hex Hdist]]. subst ρ1.
+                split; [reflexivity|split; auto].
+              * intros t' Hneq.
+	                eapply R_pres_same_π. simpl. intros Hno'. constructor.
+            }
+	          { inversion H0; subst; clear H0.
+	            destruct v2 as [rv|].
+            + pupdate_finish; split.
+              * destruct Hpre as [HI Hlive].
+                unfold I, Live, Done, Active, ALin, NoExchBy in *; simpl in *.
+                destruct HI as [Hr [Hex Hdist]]. subst ρ1.
+                destruct Hex as [Hcur Hother].
+                split.
+                -- split; [reflexivity|split; [exact Hother|exact Hdist]].
+	                -- split; [exact Hcur|exact Hdist].
+              * unfold G. split.
+                -- destruct Hpre as [HI Hlive].
+                   unfold I in *; simpl in *.
+                   destruct HI as [Hr [Hex Hdist]]. subst ρ1.
+                   destruct Hex as [Hcur Hother].
+                   split; [reflexivity|split; [exact Hother|exact Hdist]].
+                -- intros t' Hneq.
+                   eapply R_pres_same_π. simpl.
+                   intros Hno'. destruct Hno' as [_ Hneq2]. exact Hneq2.
+            + pupdate_finish; split.
+              * destruct Hpre as [HI Hlive].
+                unfold I, Live, Done, ALin, NoExchBy in *; simpl in *.
+                destruct HI as [Hr [Hex Hdist]]. subst ρ1.
+                destruct Hex as [Hcur Hother].
+                split.
+                -- split; [reflexivity|split; [exact Hother|exact Hdist]].
+                -- split; [exact Hcur|exact Hdist].
+              * unfold G. split.
+                -- destruct Hpre as [HI Hlive].
+                   unfold I in *; simpl in *.
+                   destruct HI as [Hr [Hex Hdist]]. subst ρ1.
+                   destruct Hex as [Hcur Hother].
+                   split; [reflexivity|split; [exact Hother|exact Hdist]].
+                -- intros t' Hneq.
+                   eapply R_pres_same_π. simpl.
+                   intros Hno'. destruct Hno' as [_ Hneq2]. exact Hneq2.
+            }
+	          { inversion H0; subst; clear H0.
+	            destruct v1 as [rv|].
+            + pupdate_finish; split.
+              * destruct Hpre as [HI Hlive].
+                unfold I, Live, Done, Active, ALin, NoExchBy in *; simpl in *.
+                destruct HI as [Hr [Hex Hdist]]. subst ρ1.
+                split.
+	                -- split; [reflexivity|split; constructor].
+		                -- split; [exact Hex|simpl; auto].
+              * unfold G. split.
+                -- destruct Hpre as [HI Hlive].
+                   unfold I in *; simpl in *.
+                   destruct HI as [Hr [Hex Hdist]]. subst ρ1.
+	                   split; [reflexivity|split; constructor].
+                -- intros t' Hneq.
+	                   eapply R_pres_same_π. simpl. intros Hno'. constructor.
+            + pupdate_finish; split.
+              * destruct Hpre as [HI Hlive].
+                unfold I, Live, Done, ALin, NoExchBy in *; simpl in *.
+                destruct HI as [Hr [Hex Hdist]]. subst ρ1.
+                split.
+	                -- split; [reflexivity|split; constructor].
+	                -- split; [exact Hex|simpl; auto].
+              * unfold G. split.
+                -- destruct Hpre as [HI Hlive].
+                   unfold I in *; simpl in *.
+                   destruct HI as [Hr [Hex Hdist]]. subst ρ1.
+	                   split; [reflexivity|split; constructor].
+                -- intros t' Hneq.
+	                   eapply R_pres_same_π. simpl. intros Hno'. constructor.
+            }
+        * intros [[ov|]|].
+          { eapply provable_vis_safe with
+              (P' := I //\\ Active t (push v))
+              (Q' := fun succ =>
+                match succ with
+                | OK _ => I //\\ ALin t (Semantics.ls_linr (push v) tt) //\\ NoExchBy t
+                | FAIL => I //\\ Active t (push v)
+                end);
+            try solve_conj_impl;
+            try solve_conj_stable stableDB;
+            try (intro succ; destruct succ; solve_conj_stable stableDB);
+            try solve [apply no_error].
+            + intros succ; destruct succ; solve_conj_impl.
+            + pupdate_intros_atomic.
+              pupdate_finish; split.
+              * destruct Hpre as [HI Hact].
+                unfold I in *; simpl in *.
+                destruct HI as [Hr [Hex Hdist]].
+                split; [split; [exact Hr|split; [exact Hex|exact Hdist]]|exact Hact].
+              * unfold G. split.
+	                -- destruct Hpre as [HI Hact].
+	                   unfold I in *; simpl in *.
+	                   destruct HI as [Hr [Hex Hdist]].
+	                   split; [exact Hr|split; [exact Hex|exact Hdist]].
+	                -- intros t' Hneq. eapply R_pres_same_π. simpl. auto.
+	            + intros [[]|].
+	              * pupdate_intros_atomic.
+                  {
+	                  destruct Hpre as [HI [Hlin Hno]].
+                    unfold I, Active, ALin, NoExchBy in *; simpl in *.
+                    destruct HI as [Hr [Hex Hdist]]. subst ρ1.
+                    pupdate_start.
+                    pupdate_forward t0 (InvEv (push v0)).
+                    pupdate_forward t0 (ResEv (push v0) tt).
+                    pupdate_finish.
+                    split.
+                    - split.
+	                      + split; [reflexivity|split; [eapply exch_ok_add_add_no_exch; eauto|exact Hdist]].
+                      + split.
+                        * unfold ALin; simpl. rewrite PositiveMap.gss. reflexivity.
+                        * exact Hno.
+                    - unfold G. split.
+	                      + split; [reflexivity|split; [eapply exch_ok_add_add_no_exch; eauto|exact Hdist]].
+                      + intros t' Hneq.
+                        eapply R_pres_add_add_other; [exact Hneq|].
+                        simpl. auto.
+                  }
+                * pupdate_intros_atomic.
+                  {
+                    pupdate_finish; split.
+                    - destruct Hpre as [HI Hact].
+                      unfold I in *; simpl in *.
+                      destruct HI as [Hr [Hex Hdist]].
+                      split; [split; [exact Hr|split; [exact Hex|exact Hdist]]|exact Hact].
+                    - unfold G. split.
+                      + destruct Hpre as [HI Hact].
+                        unfold I in *; simpl in *.
+                        destruct HI as [Hr [Hex Hdist]].
+                        split; [exact Hr|split; [exact Hex|exact Hdist]].
+                      + intros t' Hneq. eapply R_pres_same_π. simpl. auto.
+                  }
+	            + intros [[]|]; eapply provable_ret_safe;
+                try solve_conj_impl;
+                try solve_conj_stable stableDB.
+          }
+          { eapply provable_ret_safe;
+            try solve_conj_impl;
+            try solve_conj_stable stableDB.
+          }
+          { eapply provable_vis_safe with
+              (P' := I //\\ Active t (push v))
+              (Q' := fun succ =>
+                match succ with
+                | OK _ => I //\\ ALin t (Semantics.ls_linr (push v) tt) //\\ NoExchBy t
+                | FAIL => I //\\ Active t (push v)
+                end);
+            try solve_conj_impl;
+            try solve_conj_stable stableDB;
+            try (intro succ; destruct succ; solve_conj_stable stableDB);
+            try solve [apply no_error].
+            + intros succ; destruct succ; solve_conj_impl.
+            + pupdate_intros_atomic.
+              pupdate_finish; split.
+              * destruct Hpre as [HI Hact].
+                unfold I in *; simpl in *.
+                destruct HI as [Hr [Hex Hdist]].
+                split; [split; [exact Hr|split; [exact Hex|exact Hdist]]|exact Hact].
+              * unfold G. split.
+	                -- destruct Hpre as [HI Hact].
+	                   unfold I in *; simpl in *.
+	                   destruct HI as [Hr [Hex Hdist]].
+	                   split; [exact Hr|split; [exact Hex|exact Hdist]].
+	                -- intros t' Hneq. eapply R_pres_same_π. simpl. auto.
+	            + intros [[]|].
+                * pupdate_intros_atomic.
+                  {
+                    destruct Hpre as [HI [Hlin Hno]].
+                    unfold I, Active, ALin, NoExchBy in *; simpl in *.
+                    destruct HI as [Hr [Hex Hdist]]. subst ρ1.
+                    pupdate_start.
+                    pupdate_forward t0 (InvEv (push v0)).
+                    pupdate_forward t0 (ResEv (push v0) tt).
+                    pupdate_finish.
+                    split.
+                    - split.
+                      + split; [reflexivity|split; [eapply exch_ok_add_add_no_exch; eauto|exact Hdist]].
+                      + split.
+                        * unfold ALin; simpl. rewrite PositiveMap.gss. reflexivity.
+                        * exact Hno.
+                    - unfold G. split.
+                      + split; [reflexivity|split; [eapply exch_ok_add_add_no_exch; eauto|exact Hdist]].
+                      + intros t' Hneq.
+                        eapply R_pres_add_add_other; [exact Hneq|].
+                        simpl. auto.
+                  }
+                * pupdate_intros_atomic.
+                  {
+                    pupdate_finish; split.
+                    - destruct Hpre as [HI Hact].
+                      unfold I in *; simpl in *.
+                      destruct HI as [Hr [Hex Hdist]].
+                      split; [split; [exact Hr|split; [exact Hex|exact Hdist]]|exact Hact].
+                    - unfold G. split.
+                      + destruct Hpre as [HI Hact].
+                        unfold I in *; simpl in *.
+                        destruct HI as [Hr [Hex Hdist]].
+                        split; [exact Hr|split; [exact Hex|exact Hdist]].
+                      + intros t' Hneq. eapply R_pres_same_π. simpl. auto.
+                  }
+	            + intros [[]|]; eapply provable_ret_safe;
+                try solve_conj_impl;
+                try solve_conj_stable stableDB.
+          }
+    - exists (I //\\ Active t pop).
+      exists (fun ret => I //\\ ALin t (Semantics.ls_linr pop ret) //\\ NoExchBy t).
+      constructor.
+      + apply IGinvActive.
+      + solve_conj_impl.
+      + solve_conj_stable stableDB.
+      + intros ret. apply IGretNoExch.
+      + unfold ALin. intros ret σ0 ρ0 π0 [HI [Hlin Hno]].
+        exact Hlin.
+      + simpl. unfold pop_impl.
+        eapply provable_doloop;
+        try solve_conj_impl;
+        try solve_conj_stable stableDB.
+        eapply provable_vis_safe with
+          (P' := I //\\ Live t pop)
+          (Q' := fun other =>
+            match other with
+            | Some (Some x) => I //\\ ALin t (Semantics.ls_linr pop (Some x)) //\\ NoExchBy t
+            | _ => I //\\ Active t pop
+            end);
+        try solve_conj_impl;
+        try solve_conj_stable stableDB;
+        try (intro other; destruct other as [[ov|]|]; try destruct ov; solve_conj_stable stableDB);
+        try solve [apply no_error].
+        * intros [[ov|]|]; try destruct ov; solve_conj_impl.
+        * pupdate_intros_atomic.
+          {
+            pupdate_finish; split.
+            - destruct Hpre as [HI [Hlin Hno]].
+              unfold I, Active, Live, Done, ALin, NoExchBy in *; simpl in *.
+              split.
+              + destruct HI as [Hr _]. split; [exact Hr|split; [exact Hlin|auto]].
+              + left. exact Hlin.
+            - unfold G, R_pres, Active, Live, Done, ALin, NoExchBy.
+              split.
+              + destruct Hpre as [HI [Hlin Hno]].
+                unfold I in *; simpl in *.
+                destruct HI as [Hr _]. split; [exact Hr|split; [exact Hlin|auto]].
+              + intros t' Hneq; simpl.
+                split.
+                -- split; intro H; exact H.
+                -- split.
+                   ++ intros m [Hlin Hno]. split; [exact Hlin|congruence].
+                   ++ split.
+                      ** intros m ret Hlin. exact Hlin.
+                      ** split.
+                         --- intros m [Hlin | [ret Hlin]]; [left | right; exists ret]; exact Hlin.
+                         --- intros _. congruence.
+          }
+          {
+            destruct v1 as [w|].
+            - destruct Hpre as [HI [Hlin Hno]].
+              unfold I, Active, ALin, NoExchBy in *; simpl in *.
+              destruct HI as [Hr [Hex Hdist]]. subst ρ1.
+              pupdate_start.
+              pupdate_forward t1 (InvEv (push w)).
+              pupdate_forward t1 (ResEv (push w) tt).
+              pupdate_forward t2 (@InvEv (EStack A) (@pop A));
+                try (rewrite PositiveMap.gso by congruence;
+                     rewrite PositiveMap.gso by congruence;
+                     exact Hlin).
+              pupdate_forward t2 (@ResEv (EStack A) (@pop A) (Some w)).
+              pupdate_finish.
+              split.
+              + split.
+                * split; [reflexivity|].
+                  simpl. split.
+                  -- split.
+                     ++ rewrite PositiveMap.gso by congruence.
+                        rewrite PositiveMap.gso by congruence.
+                        rewrite PositiveMap.gss. reflexivity.
+                     ++ rewrite PositiveMap.gss. reflexivity.
+                  -- congruence.
+                * right. exists (Some w).
+                  unfold ALin; simpl. rewrite PositiveMap.gss. reflexivity.
+              + unfold G, R_pres, Active, Live, Done, ALin, NoExchBy.
+                split.
+                * split; [reflexivity|].
+                  simpl. split.
+                  -- split.
+                     ++ rewrite PositiveMap.gso by congruence.
+                        rewrite PositiveMap.gso by congruence.
+                        rewrite PositiveMap.gss. reflexivity.
+                     ++ rewrite PositiveMap.gss. reflexivity.
+                  -- congruence.
+                * intros t' Hneq.
+                  simpl.
+                  destruct (PositiveMap.E.eq_dec t' t1) as [Heq|Hne1]; subst.
+                  -- split.
+                     ++ split; intro Hnone.
+                        ** rewrite Hex in Hnone. discriminate.
+                        ** simpl in Hnone.
+                           rewrite PositiveMap.gso in Hnone by congruence.
+                           rewrite PositiveMap.gso in Hnone by congruence.
+                           rewrite PositiveMap.gss in Hnone. discriminate.
+                     ++ split.
+                        ** intros m [Hinv Hno']. contradiction.
+                        ** split.
+                           --- intros m ret Hret.
+                               simpl in Hret. rewrite Hex in Hret. discriminate.
+                           --- split.
+                               +++ intros m [Hinv | [ret Hret]].
+	                                   { destruct m as [x|].
+	                                     - right. exists tt. simpl.
+                                       simpl in Hinv. rewrite Hex in Hinv.
+                                       inversion Hinv; subst.
+	                                       rewrite PositiveMap.gso by congruence.
+	                                       rewrite PositiveMap.gso by congruence.
+	                                       rewrite PositiveMap.gss. reflexivity.
+                                     - simpl in Hinv. rewrite Hex in Hinv. discriminate. }
+                                   { simpl in Hret. rewrite Hex in Hret. discriminate. }
+                               +++ intros Hno'. contradiction.
+                  -- assert (Hne2 : t' <> t2) by congruence.
+                     simpl in *.
+                     split.
+                     ++ split; intro Hnone.
+                        ** repeat (rewrite PositiveMap.gso by congruence). exact Hnone.
+                        ** repeat (rewrite PositiveMap.gso in Hnone by congruence). exact Hnone.
+                     ++ split.
+                        ** intros m [Hinv Hno']. simpl in Hinv. split.
+                           --- simpl. repeat (rewrite PositiveMap.gso by congruence). exact Hinv.
+                           --- split; [exact Hno'|exact Hne2].
+                        ** split.
+                           --- intros m ret Hret. simpl in Hret.
+                               simpl. repeat (rewrite PositiveMap.gso by congruence). exact Hret.
+                           --- split.
+                               +++ intros m [Hinv | [ret Hret]].
+                                   { simpl in Hinv. left. simpl. repeat (rewrite PositiveMap.gso by congruence). exact Hinv. }
+                                   { simpl in Hret. right. exists ret. simpl. repeat (rewrite PositiveMap.gso by congruence). exact Hret. }
+                               +++ intros Hno'. split; [exact Hno'|exact Hne2].
+            - pupdate_finish; split.
+              + destruct Hpre as [HI [Hlin Hno]].
+                unfold I, Active, Live, Done, ALin, NoExchBy in *; simpl in *.
+                destruct HI as [Hr [Hex Hdist]].
+                split; [split; [exact Hr|split; [split; [exact Hex|exact Hlin]|congruence]]|left; exact Hlin].
+              + unfold G, R_pres, Active, Live, Done, ALin, NoExchBy.
+                split.
+                * destruct Hpre as [HI [Hlin Hno]].
+                  unfold I, Active, ALin in *; simpl in *.
+                  destruct HI as [Hr [Hex Hdist]].
+                  split; [exact Hr|split; [split; [exact Hex|exact Hlin]|congruence]].
+                * intros t' Hneq; simpl.
+                  destruct (PositiveMap.E.eq_dec t' t1) as [Heq|Hne1]; subst.
+                  -- split.
+                     ++ split; intro Hnone.
+                        ** destruct Hpre as [HI [Hlin Hno]].
+                           unfold I in HI; simpl in HI.
+                           destruct HI as [_ [Hex _]].
+                           rewrite Hex in Hnone. discriminate.
+                        ** destruct Hpre as [HI [Hlin Hno]].
+                           unfold I in HI; simpl in HI.
+                           destruct HI as [_ [Hex _]].
+                           rewrite Hex in Hnone. discriminate.
+                     ++ split.
+                        ** intros m [Hlin Hno]. contradiction.
+                        ** split.
+                           --- intros m ret Hret.
+                               destruct Hpre as [HI _].
+                               unfold I in HI; simpl in HI.
+                               destruct HI as [_ [Hex _]].
+                               simpl in Hret. rewrite Hex in Hret. discriminate.
+                           --- split.
+                               +++ intros m [Hlin | [ret Hret]].
+                                   { left; exact Hlin. }
+                                   { destruct Hpre as [HI _].
+                                     unfold I in HI; simpl in HI.
+                                     destruct HI as [_ [Hex _]].
+                                     simpl in Hret.
+                                     rewrite Hex in Hret. discriminate. }
+                               +++ intros Hno. contradiction.
+                  -- split.
+                     ++ split; intro Hnone; exact Hnone.
+                     ++ split.
+                        ** intros m [Hlin Hno]. split; [exact Hlin|split; [exact Hno|congruence]].
+                        ** split.
+                           --- intros m ret Hret. exact Hret.
+                           --- split.
+                               +++ intros m [Hlin | [ret Hret]]; [left | right; exists ret]; exact Hlin || exact Hret.
+                               +++ intros Hno. split; [exact Hno|congruence].
+          }
+        * intros ret.
+          pupdate_intros_atomic.
+          {
+            inversion H0; subst; clear H0.
+            pupdate_finish; split.
+            - destruct Hpre as [HI Hlive].
+              unfold I, Live, Done, ALin in *; simpl in *.
+              destruct HI as [Hr [Hex Hdist]]. subst ρ1.
+              split; [split; [reflexivity|split; constructor]|].
+              split; [exact Hex|simpl; auto].
+            - unfold G. split.
+              + destruct Hpre as [HI Hlive].
+                unfold I in *; simpl in *.
+                destruct HI as [Hr [Hex Hdist]]. subst ρ1.
+                split; [reflexivity|split; constructor].
+              + intros t' Hneq.
+                eapply R_pres_same_π. simpl. intros Hno'. constructor.
+          }
+          {
+            inversion H0; subst; clear H0.
+            destruct v2 as [w|].
+            - pupdate_finish; split.
+              + destruct Hpre as [HI Hlive].
+                unfold I, Live, Done, ALin, NoExchBy in *; simpl in *.
+                destruct HI as [Hr [Hex Hdist]]. subst ρ1.
+                destruct Hex as [Hcur Hother].
+                split.
+                * split; [reflexivity|split; [exact Hother|exact Hdist]].
+                * split; [exact Hcur|exact Hdist].
+              + unfold G. split.
+                * destruct Hpre as [HI Hlive].
+                  unfold I in *; simpl in *.
+                  destruct HI as [Hr [Hex Hdist]]. subst ρ1.
+                  destruct Hex as [Hcur Hother].
+                  split; [reflexivity|split; [exact Hother|exact Hdist]].
+                * intros t' Hneq.
+                  eapply R_pres_same_π. simpl.
+                  intros Hno'. destruct Hno' as [_ Hneq2]. exact Hneq2.
+            - pupdate_finish; split.
+              + destruct Hpre as [HI Hlive].
+                unfold I, Live, Done, Active, ALin, NoExchBy in *; simpl in *.
+                destruct HI as [Hr [Hex Hdist]]. subst ρ1.
+                destruct Hex as [Hcur Hother].
+                split.
+                * split; [reflexivity|split; [exact Hother|exact Hdist]].
+                * split; [exact Hcur|exact Hdist].
+              + unfold G. split.
+                * destruct Hpre as [HI Hlive].
+                  unfold I in *; simpl in *.
+                  destruct HI as [Hr [Hex Hdist]]. subst ρ1.
+                  destruct Hex as [Hcur Hother].
+                  split; [reflexivity|split; [exact Hother|exact Hdist]].
+                * intros t' Hneq.
+                  eapply R_pres_same_π. simpl.
+                  intros Hno'. destruct Hno' as [_ Hneq2]. exact Hneq2.
+          }
+          {
+            inversion H0; subst; clear H0.
+            destruct v1 as [w|].
+            - pupdate_finish; split.
+              + destruct Hpre as [HI Hlive].
+                unfold I, Live, Done, ALin, NoExchBy in *; simpl in *.
+                destruct HI as [Hr [Hex Hdist]]. subst ρ1.
+                split.
+                * split; [reflexivity|split; constructor].
+                * split; [exact Hex|simpl; auto].
+              + unfold G. split.
+                * destruct Hpre as [HI Hlive].
+                  unfold I in *; simpl in *.
+                  destruct HI as [Hr [Hex Hdist]]. subst ρ1.
+                  split; [reflexivity|split; constructor].
+                * intros t' Hneq.
+                  eapply R_pres_same_π. simpl. intros Hno'. constructor.
+            - pupdate_finish; split.
+              + destruct Hpre as [HI Hlive].
+                unfold I, Live, Done, Active, ALin, NoExchBy in *; simpl in *.
+                destruct HI as [Hr [Hex Hdist]]. subst ρ1.
+                split.
+                * split; [reflexivity|split; constructor].
+                * split; [exact Hex|simpl; auto].
+              + unfold G. split.
+                * destruct Hpre as [HI Hlive].
+                  unfold I in *; simpl in *.
+                  destruct HI as [Hr [Hex Hdist]]. subst ρ1.
+                  split; [reflexivity|split; constructor].
+	                * intros t' Hneq.
+	                  eapply R_pres_same_π. simpl. intros Hno'. constructor.
+	          }
+        * intros [[ov|]|].
+          { eapply provable_ret_safe;
+            try solve_conj_impl;
+            try solve_conj_stable stableDB.
+          }
+          { eapply provable_vis_safe with
+              (P' := I //\\ Active t pop)
+              (Q' := fun succ =>
+                match succ with
+                | OK v => I //\\ ALin t (Semantics.ls_linr pop v) //\\ NoExchBy t
+                | FAIL => I //\\ Active t pop
+                end);
+            try solve_conj_impl;
+            try solve_conj_stable stableDB;
+            try (intro succ; destruct succ; solve_conj_stable stableDB);
+            try solve [apply no_error].
+            + intros succ; destruct succ; solve_conj_impl.
+            + pupdate_intros_atomic.
+              pupdate_finish; split.
+              * destruct Hpre as [HI Hact].
+                unfold I in *; simpl in *.
+                destruct HI as [Hr [Hex Hdist]].
+                split; [split; [exact Hr|split; [exact Hex|exact Hdist]]|exact Hact].
+              * unfold G. split.
+                -- destruct Hpre as [HI Hact].
+                   unfold I in *; simpl in *.
+                   destruct HI as [Hr [Hex Hdist]].
+                   split; [exact Hr|split; [exact Hex|exact Hdist]].
+                -- intros t' Hneq. eapply R_pres_same_π. simpl. auto.
+	            + intros [retv|].
+	              * pupdate_intros_atomic.
+                {
+                  destruct Hpre as [HI [Hlin Hno]].
+                  unfold I, Active, ALin, NoExchBy in *; simpl in *.
+                  destruct HI as [Hr [Hex Hdist]]. subst ρ1.
+                  pupdate_start.
+                  pupdate_forward t0 (@InvEv (EStack A) (@pop A)).
+		                  pupdate_forward t0 (@ResEv (EStack A) (@pop A) None);
+                    try rewrite PositiveMap.gss; auto.
+                  pupdate_finish.
+                  split.
+                  - split.
+                    + split; [reflexivity|split; [eapply exch_ok_add_add_no_exch; eauto|exact Hdist]].
+                    + split.
+                      * unfold ALin; simpl. rewrite PositiveMap.gss. reflexivity.
+                      * exact Hno.
+                  - unfold G. split.
+                    + split; [reflexivity|split; [eapply exch_ok_add_add_no_exch; eauto|exact Hdist]].
+                    + intros t' Hneq.
+                      eapply R_pres_add_add_other; [exact Hneq|].
+                      simpl. auto.
+                }
+              {
+                  destruct Hpre as [HI [Hlin Hno]].
+                  unfold I, Active, ALin, NoExchBy in *; simpl in *.
+                  destruct HI as [Hr [Hex Hdist]]. subst ρ1.
+                  pupdate_start.
+                  pupdate_forward t0 (@InvEv (EStack A) (@pop A)).
+	                  pupdate_forward t0 (@ResEv (EStack A) (@pop A) (Some v));
+                    try rewrite PositiveMap.gss; auto.
+                  pupdate_finish.
+                  split.
+                  - split.
+                    + split; [reflexivity|split; [eapply exch_ok_add_add_no_exch; eauto|exact Hdist]].
+                    + split.
+                      * unfold ALin; simpl. rewrite PositiveMap.gss. reflexivity.
+                      * exact Hno.
+                  - unfold G. split.
+                    + split; [reflexivity|split; [eapply exch_ok_add_add_no_exch; eauto|exact Hdist]].
+                    + intros t' Hneq.
+                      eapply R_pres_add_add_other; [exact Hneq|].
+                      simpl. auto.
+	                }
+	              * pupdate_intros_atomic.
+                {
+	                  pupdate_finish; split.
+                  - destruct Hpre as [HI Hact].
+                    unfold I in *; simpl in *.
+                    destruct HI as [Hr [Hex Hdist]].
+                    split; [split; [exact Hr|split; [exact Hex|exact Hdist]]|exact Hact].
+                  - unfold G. split.
+                    + destruct Hpre as [HI Hact].
+                      unfold I in *; simpl in *.
+                      destruct HI as [Hr [Hex Hdist]].
+                      split; [exact Hr|split; [exact Hex|exact Hdist]].
+                    + intros t' Hneq. eapply R_pres_same_π. simpl. auto.
+                }
+            + intros [retv|]; eapply provable_ret_safe;
+              try solve_conj_impl;
+              try solve_conj_stable stableDB.
+          }
+          { eapply provable_vis_safe with
+              (P' := I //\\ Active t pop)
+              (Q' := fun succ =>
+                match succ with
+                | OK v => I //\\ ALin t (Semantics.ls_linr pop v) //\\ NoExchBy t
+                | FAIL => I //\\ Active t pop
+                end);
+            try solve_conj_impl;
+            try solve_conj_stable stableDB;
+            try (intro succ; destruct succ; solve_conj_stable stableDB);
+            try solve [apply no_error].
+            + intros succ; destruct succ; solve_conj_impl.
+            + pupdate_intros_atomic.
+              pupdate_finish; split.
+              * destruct Hpre as [HI Hact].
+                unfold I in *; simpl in *.
+                destruct HI as [Hr [Hex Hdist]].
+                split; [split; [exact Hr|split; [exact Hex|exact Hdist]]|exact Hact].
+              * unfold G. split.
+                -- destruct Hpre as [HI Hact].
+                   unfold I in *; simpl in *.
+                   destruct HI as [Hr [Hex Hdist]].
+                   split; [exact Hr|split; [exact Hex|exact Hdist]].
+                -- intros t' Hneq. eapply R_pres_same_π. simpl. auto.
+            + intros [retv|].
+              * pupdate_intros_atomic.
+                {
+                  destruct Hpre as [HI [Hlin Hno]].
+                  unfold I, Active, ALin, NoExchBy in *; simpl in *.
+                  destruct HI as [Hr [Hex Hdist]]. subst ρ1.
+                  pupdate_start.
+                  pupdate_forward t0 (@InvEv (EStack A) (@pop A)).
+	                  pupdate_forward t0 (@ResEv (EStack A) (@pop A) None);
+                    try rewrite PositiveMap.gss; auto.
+                  pupdate_finish.
+                  split.
+                  - split.
+                    + split; [reflexivity|split; [eapply exch_ok_add_add_no_exch; eauto|exact Hdist]].
+                    + split.
+                      * unfold ALin; simpl. rewrite PositiveMap.gss. reflexivity.
+                      * exact Hno.
+                  - unfold G. split.
+                    + split; [reflexivity|split; [eapply exch_ok_add_add_no_exch; eauto|exact Hdist]].
+                    + intros t' Hneq.
+                      eapply R_pres_add_add_other; [exact Hneq|].
+                      simpl. auto.
+	                }
+	              {
+	                  destruct Hpre as [HI [Hlin Hno]].
+                  unfold I, Active, ALin, NoExchBy in *; simpl in *.
+                  destruct HI as [Hr [Hex Hdist]]. subst ρ1.
+                  pupdate_start.
+                  pupdate_forward t0 (@InvEv (EStack A) (@pop A)).
+	                  pupdate_forward t0 (@ResEv (EStack A) (@pop A) (Some v));
+                    try rewrite PositiveMap.gss; auto.
+                  pupdate_finish.
+                  split.
+                  - split.
+                    + split; [reflexivity|split; [eapply exch_ok_add_add_no_exch; eauto|exact Hdist]].
+                    + split.
+                      * unfold ALin; simpl. rewrite PositiveMap.gss. reflexivity.
+                      * exact Hno.
+                  - unfold G. split.
+                    + split; [reflexivity|split; [eapply exch_ok_add_add_no_exch; eauto|exact Hdist]].
+                    + intros t' Hneq.
+                      eapply R_pres_add_add_other; [exact Hneq|].
+                      simpl. auto.
+                }
+              * pupdate_intros_atomic.
+                {
+                  pupdate_finish; split.
+                  - destruct Hpre as [HI Hact].
+                    unfold I in *; simpl in *.
+                    destruct HI as [Hr [Hex Hdist]].
+                    split; [split; [exact Hr|split; [exact Hex|exact Hdist]]|exact Hact].
+                  - unfold G. split.
+                    + destruct Hpre as [HI Hact].
+                      unfold I in *; simpl in *.
+                      destruct HI as [Hr [Hex Hdist]].
+                      split; [exact Hr|split; [exact Hex|exact Hdist]].
+                    + intros t' Hneq. eapply R_pres_same_π. simpl. auto.
+                }
+            + intros [retv|]; eapply provable_ret_safe;
+              try solve_conj_impl;
+              try solve_conj_stable stableDB.
+          }
+    - unfold I. simpl. split; [reflexivity|split; constructor].
+  Defined.
+End EBStackImpl.
